iso: Checkpoint cache msg routing logic

examples/dynamic_isolation/Memory.v
@@ -10,7 +10,542 @@ Require Import DynamicIsolation.External.
 Require Import DynamicIsolation.Tactics.
 Require Import DynamicIsolation.Interfaces.
 
-Module Memory <: Memory_sig External.
+(* Heavily inspired by http://csg.csail.mit.edu/6.175/labs/project-part1.html *)
+
+Module CacheTypes.
+  Import Common.
+
+  Definition MSI :=
+    {| enum_name := "MSI";
+       enum_members := vect_of_list ["M"; "S"; "I"];
+       enum_bitpatterns := vect_of_list [Ob~0~0; Ob~0~1; Ob~1~0] |}.
+
+  Definition cache_type :=
+    {| enum_name := "cache_type";
+       enum_members := vect_of_list ["imem"; "dmem"];
+       enum_bitpatterns := vect_of_list [Ob~0; Ob~1] |}.
+
+
+  Definition cache_mem_req :=
+    {| struct_name := "cache_mem_req";
+       struct_fields := [("core_id" , bits_t 1);
+                         ("cache_type", enum_t cache_type);
+                         ("addr"    , addr_t);
+                         ("MSI_state"   , enum_t MSI)] |}.
+
+  Definition cache_mem_resp :=
+    {| struct_name := "cache_mem_resp";
+       struct_fields := [("core_id"   , bits_t 1);
+                         ("cache_type", enum_t cache_type);
+                         ("addr"      , addr_t);
+                         ("MSI_state" , enum_t MSI);
+                         ("data"      , maybe (data_t))
+                        ] |}.
+
+  Module FifoCacheMemReq <: Fifo.
+    Definition T:= struct_t cache_mem_req.
+  End FifoCacheMemReq.
+  Module CacheMemReq := Fifo1 FifoMemReq.
+
+  Module FifoCacheMemResp <: Fifo.
+    Definition T:= struct_t cache_mem_resp.
+  End FifoCacheMemResp.
+  Module CacheMemResp := Fifo1 FifoMemResp.
+
+  Definition cache_mem_msg_tag :=
+    {| enum_name := "cache_mem_msg_tag";
+       enum_members := vect_of_list ["Req"; "Resp"];
+       enum_bitpatterns := vect_of_list [Ob~0; Ob~1] |}.
+
+  (* NOTE: This should be a union type if one existed. What is the best way to encode this? *)
+  Definition cache_mem_msg :=
+    {| struct_name := "cache_mem_msg";
+       struct_fields := [("type", enum_t cache_mem_msg_tag );
+                         ("req" , struct_t cache_mem_req);
+                         ("resp" , struct_t cache_mem_resp)
+                        ] |}.
+
+End CacheTypes.
+
+Module MessageFifo1.
+  Import CacheTypes.
+
+  (* A message FIFO has two enqueue methods (enq_resp and enq_req), and behaves such that a request
+   * never blocks a response.
+   *)
+  Inductive reg_t :=
+  | reqQueue (state: CacheMemReq.reg_t)
+  | respQueue (state: CacheMemResp.reg_t).
+
+  Definition R r :=
+    match r with
+    | reqQueue s => CacheMemReq.R s
+    | respQueue s => CacheMemResp.R s
+    end.
+
+  Definition r idx : R idx :=
+    match idx with
+    | reqQueue s => CacheMemReq.r s
+    | respQueue s => CacheMemResp.r s
+    end.
+
+  Definition enq_resp : UInternalFunction reg_t empty_ext_fn_t :=
+    {{ fun enq_resp (resp: struct_t cache_mem_resp) : bits_t 0 =>
+         respQueue.(CacheMemResp.enq)()
+    }}.
+
+  Definition enq_req : UInternalFunction reg_t empty_ext_fn_t :=
+    {{ fun enq_req (resp: struct_t cache_mem_req) : bits_t 0 =>
+         reqQueue.(CacheMemReq.enq)()
+    }}.
+
+  Definition has_resp : UInternalFunction reg_t empty_ext_fn_t :=
+    {{ fun has_resp () : bits_t 1 =>
+         respQueue.(CacheMemResp.can_deq)()
+    }}.
+
+  Definition has_req : UInternalFunction reg_t empty_ext_fn_t :=
+    {{ fun has_req () : bits_t 1 =>
+         reqQueue.(CacheMemReq.can_deq)()
+    }}.
+
+  Definition not_empty : UInternalFunction reg_t empty_ext_fn_t :=
+    {{ fun not_empty () : bits_t 1 =>
+         has_resp() || has_req()
+    }}.
+
+  (* TODO: ugly; peek returns a maybe type *)
+  Definition peek : UInternalFunction reg_t empty_ext_fn_t :=
+    {{ fun peek () : maybe (struct_t cache_mem_msg) =>
+         if has_resp() then
+           let resp_opt := respQueue.(CacheMemResp.peek)() in
+           let msg := struct cache_mem_msg {| type := enum cache_mem_msg_tag {| Resp |};
+                                              resp := get(resp_opt, data)
+                                           |} in
+           {valid (struct_t cache_mem_msg)}(msg)
+         else if has_req() then
+           let req_opt := reqQueue.(CacheMemReq.peek)() in
+           let msg := struct cache_mem_msg {| type := enum cache_mem_msg_tag {| Req |};
+                                              resp := get(req_opt, data)
+                                           |} in
+           {valid (struct_t cache_mem_msg)}(msg)
+         else
+           {invalid (struct_t cache_mem_msg)}()
+    }}.
+
+  Definition deq : UInternalFunction reg_t empty_ext_fn_t :=
+    {{ fun deq () : struct_t cache_mem_msg =>
+       guard (not_empty());
+       if has_resp() then
+           let resp_opt := respQueue.(CacheMemResp.peek)() in
+           struct cache_mem_msg {| type := enum cache_mem_msg_tag {| Resp |};
+                                   resp := get(resp_opt, data)
+                                |}
+       else
+           let req_opt := reqQueue.(CacheMemReq.peek)() in
+           struct cache_mem_msg {| type := enum cache_mem_msg_tag {| Req |};
+                                   resp := get(req_opt, data)
+                                |}
+   }}.
+
+  Instance FiniteType_reg_t : FiniteType reg_t := _.
+
+  (* TODO: Test this. *)
+End MessageFifo1.
+
+Module WIPMemory <: Memory_sig External.
+  Import Common.
+
+  (* This memory has two L1 I&D caches, a message router, and protocol processor, and the main memory.
+   * TODO: next we will add a L2 cache.
+   *)
+
+  (* TODO: In theory we would do this in a more modular way, but we simplify for now.
+   *)
+  Inductive internal_reg_t' : Type :=
+  | core0IToRouter (state: MessageFifo1.reg_t)
+  | core0DToRouter (state: MessageFifo1.reg_t)
+  | core1IToRouter (state: MessageFifo1.reg_t)
+  | core1DToRouter (state: MessageFifo1.reg_t)
+  | RouterToCore0I (state: MessageFifo1.reg_t)
+  | RouterToCore0D (state: MessageFifo1.reg_t)
+  | RouterToCore1I (state: MessageFifo1.reg_t)
+  | RouterToCore1D (state: MessageFifo1.reg_t)
+  | RouterToProto (state: MessageFifo1.reg_t)
+  | ProtoToRouter (state: MessageFifo1.reg_t)
+  | routerTiebreaker (* To implement round-robin fairness *)
+  .
+
+  Definition internal_reg_t := internal_reg_t'.
+
+  Definition R_internal (idx: internal_reg_t) : type :=
+    match idx with
+    | core0IToRouter st => MessageFifo1.R st
+    | core0DToRouter st => MessageFifo1.R st
+    | core1IToRouter st => MessageFifo1.R st
+    | core1DToRouter st => MessageFifo1.R st
+    | RouterToCore0I st => MessageFifo1.R st
+    | RouterToCore0D st => MessageFifo1.R st
+    | RouterToCore1I st => MessageFifo1.R st
+    | RouterToCore1D st => MessageFifo1.R st
+    | RouterToProto st => MessageFifo1.R st
+    | ProtoToRouter st => MessageFifo1.R st
+    | routerTiebreaker => bits_t 2
+    end.
+
+  Definition r_internal (idx: internal_reg_t) : R_internal idx :=
+    match idx with
+    | core0IToRouter st => MessageFifo1.r st
+    | core0DToRouter st => MessageFifo1.r st
+    | core1IToRouter st => MessageFifo1.r st
+    | core1DToRouter st => MessageFifo1.r st
+    | RouterToCore0I st => MessageFifo1.r st
+    | RouterToCore0D st => MessageFifo1.r st
+    | RouterToCore1I st => MessageFifo1.r st
+    | RouterToCore1D st => MessageFifo1.r st
+    | RouterToProto st => MessageFifo1.r st
+    | ProtoToRouter st => MessageFifo1.r st
+    | routerTiebreaker => Bits.zero
+    end.
+
+  Instance FiniteType_internal_reg_t : FiniteType internal_reg_t := _.
+
+  Inductive reg_t :=
+  | toIMem0 (state: MemReq.reg_t)
+  | toIMem1 (state: MemReq.reg_t)
+  | toDMem0 (state: MemReq.reg_t)
+  | toDMem1 (state: MemReq.reg_t)
+  | fromIMem0 (state: MemResp.reg_t)
+  | fromIMem1 (state: MemResp.reg_t)
+  | fromDMem0 (state: MemResp.reg_t)
+  | fromDMem1 (state: MemResp.reg_t)
+  | internal (r: internal_reg_t)
+  .
+
+  Definition R (idx: reg_t) :=
+    match idx with
+    | toIMem0 st => MemReq.R st
+    | toIMem1 st => MemReq.R st
+    | toDMem0 st => MemReq.R st
+    | toDMem1 st => MemReq.R st
+    | fromIMem0 st => MemResp.R st
+    | fromIMem1 st => MemResp.R st
+    | fromDMem0 st => MemResp.R st
+    | fromDMem1 st => MemResp.R st
+    | internal st => R_internal st
+    end.
+
+  Definition r idx : R idx :=
+    match idx with
+    | toIMem0 st => MemReq.r st
+    | toIMem1 st => MemReq.r st
+    | toDMem0 st => MemReq.r st
+    | toDMem1 st => MemReq.r st
+    | fromIMem0 st => MemResp.r st
+    | fromIMem1 st => MemResp.r st
+    | fromDMem0 st => MemResp.r st
+    | fromDMem1 st => MemResp.r st
+    | internal st => r_internal st
+    end.
+
+  Definition ext_fn_t := External.ext_fn_t.
+  Definition Sigma := External.Sigma.
+  Definition rule := rule R Sigma.
+  (* Definition sigma := External.sigma. *)
+
+  Definition MMIO_UART_ADDRESS := Ob~0~1~0~0~0~0~0~0~0~0~0~0~0~0~0~0~0~0~0~0~0~0~0~0~0~0~0~0~0~0~0~0.
+  Definition MMIO_LED_ADDRESS  := Ob~0~1~0~0~0~0~0~0~0~0~0~0~0~0~0~0~0~0~0~0~0~0~0~0~0~0~0~0~0~1~0~0.
+
+
+  Notation "'__internal__' instance " :=
+    (fun reg => internal ((instance) reg)) (in custom koika at level 1, instance constr at level 99).
+  Notation "'(' instance ').(' method ')' args" :=
+    (USugar (UCallModule instance _ method args))
+      (in custom koika at level 1, method constr, args custom koika_args at level 99).
+
+  Import External.
+  Import CacheTypes.
+
+  (* ===================== Message routing rules ============================== *)
+  Definition router_memToCore : uaction reg_t ext_fn_t :=
+    {{ let msg := (__internal__ ProtoToRouter).(MessageFifo1.deq)() in
+       if (get(msg, type) == enum cache_mem_msg_tag {| Req |}) then
+         let req := get(msg, req) in
+         if (get(req, core_id) == Ob~0) then
+           if (get(req, cache_type) == enum cache_type {| imem |}) then
+             (__internal__ RouterToCore0I).(MessageFifo1.enq_req)(req)
+           else
+             (__internal__ RouterToCore0D).(MessageFifo1.enq_req)(req)
+         else
+           if (get(req, cache_type) == enum cache_type {| imem |}) then
+             (__internal__ RouterToCore1I).(MessageFifo1.enq_req)(req)
+           else
+             (__internal__ RouterToCore1D).(MessageFifo1.enq_req)(req)
+       else (* Resp *)
+         let resp := get(msg, resp) in
+         if (get(resp, core_id) == Ob~0) then
+           if (get(req, cache_type) == enum cache_type {| imem |}) then
+             (__internal__ RouterToCore0I).(MessageFifo1.enq_resp)(resp)
+           else
+             (__internal__ RouterToCore0D).(MessageFifo1.enq_resp)(resp)
+         else
+           if (get(resp, cache_type) == enum cache_type {| imem |}) then
+             (__internal__ RouterToCore1I).(MessageFifo1.enq_resp)(resp)
+           else
+             (__internal__ RouterToCore1D).(MessageFifo1.enq_resp)(resp)
+    }}.
+
+  Definition router_getResp : UInternalFunction reg_t empty_ext_fn_t :=
+    {{ fun router_getResp (tiebreaker : bits_t 2) : maybe (struct_t cache_mem_msg) =>
+           match tiebreaker with
+           | Ob~0~0 =>
+               if ((__internal__ core0IToRouter).(MessageFifo1.has_resp)()) then
+                 {valid (struct_t cache_mem_msg)}((__internal__ core0IToRouter).(MessageFifo1.deq)())
+               else
+                 {invalid (struct_t cache_mem_msg)}()
+           | Ob~0~1 =>
+               if ((__internal__ core0DToRouter).(MessageFifo1.has_resp)()) then
+                 {valid (struct_t cache_mem_msg)}((__internal__ core0DToRouter).(MessageFifo1.deq)())
+               else
+                 {invalid (struct_t cache_mem_msg)}()
+           | Ob~1~0 =>
+               if ((__internal__ core1IToRouter).(MessageFifo1.has_resp)()) then
+                 {valid (struct_t cache_mem_msg)}((__internal__ core1IToRouter).(MessageFifo1.deq)())
+               else
+                 {invalid (struct_t cache_mem_msg)}()
+           | Ob~1~1 =>
+               if ((__internal__ core1DToRouter).(MessageFifo1.has_resp)()) then
+                 {valid (struct_t cache_mem_msg)}((__internal__ core1DToRouter).(MessageFifo1.deq)())
+               else
+                 {invalid (struct_t cache_mem_msg)}()
+           return default : {invalid (struct_t cache_mem_msg)}()
+           end
+    }}.
+
+  Definition router_getReq : UInternalFunction reg_t empty_ext_fn_t :=
+    {{ fun router_getReq (tiebreaker : bits_t 2) : maybe (struct_t cache_mem_msg) =>
+           match tiebreaker with
+           | Ob~0~0 =>
+               if (!(__internal__ core0IToRouter).(MessageFifo1.has_resp)() &&
+                    (__internal__ core0IToRouter).(MessageFifo1.has_req)()) then
+                 {valid (struct_t cache_mem_msg)}((__internal__ core0IToRouter).(MessageFifo1.deq)())
+               else
+                 {invalid (struct_t cache_mem_msg)}()
+           | Ob~0~1 =>
+               if (!(__internal__ core0DToRouter).(MessageFifo1.has_resp)() &&
+                    (__internal__ core0DToRouter).(MessageFifo1.has_req)()) then
+                 {valid (struct_t cache_mem_msg)}((__internal__ core0DToRouter).(MessageFifo1.deq)())
+               else
+                 {invalid (struct_t cache_mem_msg)}()
+           | Ob~1~0 =>
+               if (!(__internal__ core1IToRouter).(MessageFifo1.has_resp)() &&
+                    (__internal__ core1IToRouter).(MessageFifo1.has_req)()) then
+                 {valid (struct_t cache_mem_msg)}((__internal__ core1IToRouter).(MessageFifo1.deq)())
+               else
+                 {invalid (struct_t cache_mem_msg)}()
+           | Ob~1~1 =>
+               if (!(__internal__ core1DToRouter).(MessageFifo1.has_resp)() &&
+                    (__internal__ core1DToRouter).(MessageFifo1.has_req)()) then
+                 {valid (struct_t cache_mem_msg)}((__internal__ core1DToRouter).(MessageFifo1.deq)())
+               else
+                 {invalid (struct_t cache_mem_msg)}()
+           return default : {invalid (struct_t cache_mem_msg)}()
+           end
+    }}.
+
+  (* TODO: very ugly... *)
+  (* ======= Search for responses, starting with tiebreaker ====== *)
+  Definition router_searchResponses : UInternalFunction reg_t empty_ext_fn_t :=
+    {{ fun router_searchResponses (tiebreaker : bits_t 2) : maybe (struct_t cache_mem_msg) =>
+         let foundMsg := Ob~0 in
+         let msg := {invalid (struct_t cache_mem_msg)}() in
+         when (!foundMsg) do (
+           let curResp := router_getResp (tiebreaker) in
+            when (get(curResp, valid)) do (
+              set foundMsg := Ob~1;
+              set msg := get(curResp, data);
+              write0(internal routerTiebreaker, tiebreaker + |2`d1|)
+            )
+          );
+         when (!foundMsg) do (
+           let curResp := router_getResp (tiebreaker+|2`d1|) in
+           when (get(curResp, valid)) do (
+             set foundMsg := Ob~1;
+             set msg := get(curResp, data);
+             write0(internal routerTiebreaker, tiebreaker + |2`d2|)
+           )
+         );
+         when (!foundMsg) do (
+           let curResp := router_getResp (tiebreaker+|2`d2|) in
+           when (get(curResp, valid)) do (
+             set foundMsg := Ob~1;
+             set msg := get(curResp, data);
+             write0(internal routerTiebreaker, tiebreaker + |2`d3|)
+           )
+         );
+         when (!foundMsg) do (
+           let curResp := router_getResp (tiebreaker+|2`d3|) in
+           when (get(curResp, valid)) do (
+             set foundMsg := Ob~1;
+             set msg := get(curResp, data);
+             write0(internal routerTiebreaker, tiebreaker + |2`d4|)
+           )
+         )
+     }}.
+
+  (* ======= Search for responses, starting with tiebreaker ====== *)
+  Definition router_searchRequests : UInternalFunction reg_t empty_ext_fn_t :=
+    {{ fun router_searchRequests (tiebreaker : bits_t 2) : maybe (struct_t cache_mem_msg) =>
+         let foundMsg := Ob~0 in
+         let msg := {invalid (struct_t cache_mem_msg)}() in
+         when (!foundMsg) do (
+           let curReq := router_getReq (tiebreaker) in
+            when (get(curReq, valid)) do (
+              set foundMsg := Ob~1;
+              set msg := get(curReq, data);
+              write0(internal routerTiebreaker, tiebreaker + |2`d1|)
+            )
+          );
+         when (!foundMsg) do (
+           let curReq := router_getReq (tiebreaker+|2`d1|) in
+           when (get(curReq, valid)) do (
+             set foundMsg := Ob~1;
+             set msg := get(curReq, data);
+             write0(internal routerTiebreaker, tiebreaker + |2`d2|)
+           )
+         );
+         when (!foundMsg) do (
+           let curReq := router_getReq (tiebreaker+|2`d2|) in
+           when (get(curReq, valid)) do (
+             set foundMsg := Ob~1;
+             set msg := get(curReq, data);
+             write0(internal routerTiebreaker, tiebreaker + |2`d3|)
+           )
+         );
+         when (!foundMsg) do (
+           let curReq := router_getReq (tiebreaker+|2`d3|) in
+           when (get(curReq, valid)) do (
+             set foundMsg := Ob~1;
+             set msg := get(curReq, data);
+             write0(internal routerTiebreaker, tiebreaker + |2`d4|)
+           )
+         )
+     }}.
+
+  Definition router_coreToMem : uaction reg_t ext_fn_t :=
+    {{ let tiebreaker := read0(internal routerTiebreaker) in
+       (* Search for requests, starting with tiebreaker *)
+       let msg := router_searchResponses (tiebreaker) in
+       if (get(msg, valid)) then
+         (* enqueue *)
+         (__internal__ RouterToProto).(MessageFifo1.enq_resp)(get(msg,resp))
+       else
+       (* Search for responses, starting with tiebreaker *)
+         let msg := router_searchRequests (tiebreaker) in
+         if (get(msg,valid)) then
+           (__internal__ RouterToProto).(MessageFifo1.enq_req)(get(msg,req))
+         else
+           write0(internal routerTiebreaker, tiebreaker + |2`d1|)
+    }}.
+
+  Definition memoryBus (m: memory) : UInternalFunction reg_t ext_fn_t :=
+    {{ fun memoryBus (get_ready: bits_t 1) (put_valid: bits_t 1) (put_request: struct_t mem_req) : struct_t mem_output =>
+         `match m with
+          | imem => {{ extcall (ext_mem m) (struct mem_input {|
+                        get_ready := get_ready;
+                        put_valid := put_valid;
+                        put_request := put_request |}) }}
+          | dmem => {{ let addr := get(put_request, addr) in
+                      let byte_en := get(put_request, byte_en) in
+                      let is_write := byte_en == Ob~1~1~1~1 in
+
+                      let is_uart := addr == #MMIO_UART_ADDRESS in
+                      let is_uart_read := is_uart && !is_write in
+                      let is_uart_write := is_uart && is_write in
+
+                      let is_led := addr == #MMIO_LED_ADDRESS in
+                      let is_led_write := is_led && is_write in
+
+                      let is_mem := !is_uart && !is_led in
+
+                      if is_uart_write then
+                        let char := get(put_request, data)[|5`d0| :+ 8] in
+                        let may_run := get_ready && put_valid && is_uart_write in
+                        let ready := extcall ext_uart_write (struct (Maybe (bits_t 8)) {|
+                          valid := may_run; data := char |}) in
+                        struct mem_output {| get_valid := may_run && ready;
+                                             put_ready := may_run && ready;
+                                             get_response := struct mem_resp {|
+                                               byte_en := byte_en; addr := addr;
+                                               data := |32`d0| |} |}
+
+                      else if is_uart_read then
+                        let may_run := get_ready && put_valid && is_uart_read in
+                        let opt_char := extcall ext_uart_read (may_run) in
+                        let ready := get(opt_char, valid) in
+                        struct mem_output {| get_valid := may_run && ready;
+                                             put_ready := may_run && ready;
+                                             get_response := struct mem_resp {|
+                                               byte_en := byte_en; addr := addr;
+                                               data := zeroExtend(get(opt_char, data), 32) |} |}
+
+                      else if is_led then
+                        let on := get(put_request, data)[|5`d0|] in
+                        let may_run := get_ready && put_valid && is_led_write in
+                        let current := extcall ext_led (struct (Maybe (bits_t 1)) {|
+                          valid := may_run; data := on |}) in
+                        let ready := Ob~1 in
+                        struct mem_output {| get_valid := may_run && ready;
+                                             put_ready := may_run && ready;
+                                             get_response := struct mem_resp {|
+                                               byte_en := byte_en; addr := addr;
+                                               data := zeroExtend(current, 32) |} |}
+
+                      else
+                        extcall (ext_mem m) (struct mem_input {|
+                          get_ready := get_ready && is_mem;
+                          put_valid := put_valid && is_mem;
+                          put_request := put_request |})
+                   }}
+          end` }}.
+
+  Definition mem (m: memory) : uaction reg_t ext_fn_t :=
+    let fromMem := match m with imem => fromIMem0 | dmem => fromDMem0 end in
+    let toMem := match m with imem => toIMem0 | dmem => toDMem0 end in
+    {{
+        let get_ready := fromMem.(MemResp.can_enq)() in
+        let put_request_opt := toMem.(MemReq.peek)() in
+        let put_request := get(put_request_opt, data) in
+        let put_valid := get(put_request_opt, valid) in
+        let mem_out := {memoryBus m}(get_ready, put_valid, put_request) in
+        (when (get_ready && get(mem_out, get_valid)) do fromMem.(MemResp.enq)(get(mem_out, get_response)));
+        (when (put_valid && get(mem_out, put_ready)) do ignore(toMem.(MemReq.deq)()))
+    }}.
+
+  Definition tc_imem := tc_rule R Sigma (mem imem) <: rule.
+  Definition tc_dmem := tc_rule R Sigma (mem dmem) <: rule.
+
+  Inductive rule_name_t' :=
+  | Imem
+  | Dmem
+  .
+
+  Definition rule_name_t := rule_name_t'.
+
+  Definition rules (rl: rule_name_t) : rule :=
+    match rl with
+    | Imem           => tc_imem
+    | Dmem           => tc_dmem
+    end.
+
+  Definition schedule : scheduler :=
+    Imem |> Dmem |> done.
+
+  Instance FiniteType_reg_t : FiniteType reg_t := _.
+End WIPMemory.
+
+
+Module SimpleMemory <: Memory_sig External.
   Import Common.
 
   (* TOOD: Silly workaround due to extraction issues: https://github.com/coq/coq/issues/12124 *)
@@ -175,4 +710,4 @@ Module Memory <: Memory_sig External.
 
   Instance FiniteType_internal_reg_t : FiniteType internal_reg_t := _.
   Instance FiniteType_reg_t : FiniteType reg_t := _.
-End Memory.
+End SimpleMemory.
