examples/dynamic_isolation/rv32.v
@@ -17,7 +17,7 @@ End Params1.
 Module Core0_rv32i := RV32I EnclaveParams Params0.
 Module Core0_rv32e := RV32E EnclaveParams Params0.
 Module Core1 := EmptyCore External EnclaveParams Params1.
-Module Mem := Memory.
+Module Mem := WIPMemory.
 
 (* TODO: modularize *)
 
